Compiler.thy
@@ -3,7 +3,7 @@ theory Compiler
 begin
 
 definition complete_compile :: "nexpr \<Rightarrow> byte_code list" where
-  "complete_compile e = flatten_code (compile (convert e) [])"
+  "complete_compile = flatten_code \<circ> compile \<circ> convert"
 
 theorem tc_terminationn: "typechecks e \<Longrightarrow> complete_compile e = cd \<Longrightarrow> 
   \<exists>v. valn v \<and> iter (\<leadsto>\<^sub>n) e v \<and> 
@@ -16,30 +16,29 @@ proof -
   then obtain v\<^sub>d where VD: "vald v\<^sub>d \<and> iter (\<leadsto>\<^sub>d) (convert e) v\<^sub>d" by fastforce
   with TN obtain v\<^sub>n where EN: "iter (\<leadsto>\<^sub>n) e v\<^sub>n \<and> v\<^sub>d = convert v\<^sub>n" by fastforce
   with VD have VN: "valn v\<^sub>n" by (metis convert_val_back)
-  with VD EN TD have ES: "iter (\<leadsto>\<^sub>s) (SS [] (convert e)) (SS [] (convert v\<^sub>n))" by simp
-  from TD have TC: "CSE [] [] (convert e) :\<^sub>c t" 
-    by (metis tcc_state_ev tcc_nil tcc_snil latest_environment.simps(1))
-  with ES VD EN obtain c where EC: "iter (\<leadsto>\<^sub>c) (CSE [] [] (convert e)) (CSC [] c) \<and> 
+  with VD EN TD have ES: "iter (\<leadsto>\<^sub>s) (SS [FReturn] (convert e)) (SS [] (convert v\<^sub>n))" by simp
+  from TD have TC: "CSE [CReturn []] [] (convert e) :\<^sub>c t" 
+    by (metis tcc_state_ev tcc_nil tcc_snil tcc_scons_ret latest_environment.simps(4))
+  with ES VD EN obtain c where EC: "iter (\<leadsto>\<^sub>c) (CSE [CReturn []] [] (convert e)) (CSC [] c) \<and> 
     declosure c = convert v\<^sub>n" by fastforce
   with VN have VC: "print_closure c = print_nexpr v\<^sub>n" by simp
-  from TC EC have "iter (\<leadsto>\<^sub>t) (compile_state (CSE [] [] (convert e))) (compile_state (CSC [] c))" 
-    by (metis iter_completet)
-  hence ET: "iter (\<leadsto>\<^sub>t) (TS [] [[]] (compile (convert e) [])) (TS [compile_closure c] [] [])" 
+  from TC EC have "iter (\<leadsto>\<^sub>t) (compile_state (CSE [CReturn []] [] (convert e))) 
+    (compile_state (CSC [] c))" by (metis iter_completet)
+  hence ET: "iter (\<leadsto>\<^sub>t) (TS [] [[]] (compile (convert e))) (TS [compile_closure c] [] [])" 
     by simp
   assume "complete_compile e = cd"
-  hence C: "flatten_code (compile (convert e) []) = cd" by (simp add: complete_compile_def)
-  hence "unflatten_code cd (length cd) = compile (convert e) []" by auto
-  hence UB: "unflatten_state (BS [] [[]] [length cd] cd) = TS [] [[]] (compile (convert e) [])" 
-    by simp
-  from C have "orderly_state (BS [] [[]] [length cd] cd)" by autox
+  hence C: "flatten_code (compile (convert e)) = cd" by (simp add: complete_compile_def)
+  hence "unflatten_code cd (length cd) = compile (convert e)" by auto
+  hence UB: "unflatten_state (BS [] [[]] [length cd] cd) = TS [] [[]] (compile (convert e))" by simp
+  from C have "orderly_state (BS [] [[]] [length cd] cd)" by auto
   with ET UB obtain v\<^sub>b where EB: 
     "iter (\<leadsto>\<^sub>b) (BS [] [[]] [length cd] cd) (BS [v\<^sub>b] [] [] cd) \<and> 
       compile_closure c = unflatten_closure cd v\<^sub>b" 
     by (metis evalb_end byte_code_state.sel(4))
-  hence "print_bclosure v\<^sub>b = print_tclosure (compile_closure c)" by simpx
+  hence "print_bclosure v\<^sub>b = print_tclosure (compile_closure c)" by simp
   with VC have VB: "print_bclosure v\<^sub>b = print_nexpr v\<^sub>n" by simp
   from EB obtain \<Sigma>\<^sub>h' where EH: "iter (\<leadsto>\<^sub>h) (HS hempty [] [[]] [length cd] cd) \<Sigma>\<^sub>h' \<and> 
-    BS [v\<^sub>b] [] [] cd = unheap \<Sigma>\<^sub>h'" by fastforcex
+    BS [v\<^sub>b] [] [] cd = unheap \<Sigma>\<^sub>h'" by fastforce
   then obtain h\<^sub>h v\<^sub>h where SH: "\<Sigma>\<^sub>h' = HS h\<^sub>h [v\<^sub>h] [] [] cd \<and> v\<^sub>b = unheap_closure h\<^sub>h v\<^sub>h" 
     using unheap_backwards by blast
   with VB have VH: "print_hclosure (hlookup h\<^sub>h v\<^sub>h) = print_nexpr v\<^sub>n" by simp
@@ -49,7 +48,7 @@ proof -
   with SH have "flatten \<Sigma>\<^sub>h' = FS h\<^sub>f [mp v\<^sub>h] [] [] cd" by simp
   with EH FS HS have EF: "iter (\<leadsto>\<^sub>f) (FS hempty [] [[]] [length cd] cd) (FS h\<^sub>f [mp v\<^sub>h] [] [] cd)"
     by (metis completef_iter)
-  from EH have "heap_structured \<Sigma>\<^sub>h'" by fastforcex
+  from EH have "heap_structured \<Sigma>\<^sub>h'" by fastforce
   with SH have "hcontains h\<^sub>h v\<^sub>h" by simp
   with HC have "get_closure h\<^sub>f (mp v\<^sub>h) = flatten_closure mp (hlookup h\<^sub>h v\<^sub>h)" 
     by (metis get_closure_flatten)
